CertifyingDatalog/Datalog/Grounding.lean
@@ -2,22 +2,42 @@ import CertifyingDatalog.Basic
 import CertifyingDatalog.Datalog.Basic
 
 @[ext]
-structure GroundAtom (τ: Signature) [DecidableEq τ.vars] [DecidableEq τ.relationSymbols] [DecidableEq τ.constants] [Hashable τ.constants] [Hashable τ.vars] [Hashable τ.relationSymbols]
+structure GroundAtom (τ: Signature)
 where
   symbol: τ.relationSymbols
   atom_terms: List (τ.constants)
   term_length: atom_terms.length = τ.relationArity symbol
-  deriving DecidableEq, Hashable
+
+instance {τ: Signature} [DecidableEq τ.vars] [DecidableEq τ.relationSymbols] [DecidableEq τ.constants] : DecidableEq (GroundAtom τ) :=
+  fun l r =>
+    if h: l.symbol = r.symbol
+    then
+      if h': l.atom_terms = r.atom_terms
+      then isTrue (by ext; exact h; simp [h'])
+      else isFalse (by by_contra p; rw[p] at h'; contradiction)
+    else isFalse (by by_contra p; rw[p] at h; contradiction)
+
+instance {τ: Signature} [Hashable τ.vars] [Hashable τ.relationSymbols] [Hashable τ.constants] : Hashable (GroundAtom τ) where
+  hash :=
+    fun a => mixHash (hash a.symbol) (hash a.atom_terms)
 
 @[ext]
-structure GroundRule (τ: Signature) [DecidableEq τ.vars] [DecidableEq τ.relationSymbols] [DecidableEq τ.constants] [Hashable τ.constants] [Hashable τ.vars] [Hashable τ.relationSymbols] where
+structure GroundRule (τ: Signature) where
   head: GroundAtom τ
   body: List (GroundAtom τ)
-  deriving DecidableEq
+
+instance {τ: Signature} [DecidableEq τ.vars] [DecidableEq τ.relationSymbols] [DecidableEq τ.constants] : DecidableEq (GroundRule τ) :=
+  fun l r =>
+    if h:l.head = r.head
+    then
+      if h':l.body = r.body
+      then isTrue (by ext; rw[h]; rw[h]; rw[h'])
+      else isFalse (by by_contra p; rw [p] at h'; contradiction)
+    else isFalse (by by_contra p; rw[p] at h; contradiction)
 
 abbrev Grounding (τ: Signature) := τ.vars → τ.constants
 
-variable {τ: Signature} [DecidableEq τ.vars] [DecidableEq τ.relationSymbols] [DecidableEq τ.constants] [Hashable τ.constants] [Hashable τ.vars] [Hashable τ.relationSymbols]
+variable {τ: Signature}
 
 namespace GroundAtom
   def toAtom (ga: GroundAtom τ): Atom τ:= {symbol:=ga.symbol, atom_terms:= List.map Term.constant ga.atom_terms,term_length := by rw [List.length_map]; exact ga.term_length}
@@ -25,67 +45,64 @@ namespace GroundAtom
   lemma eq_iff_toAtom_eq (a1 a2: GroundAtom τ): a1 = a2 ↔ a1.toAtom = a2.toAtom :=
   by
     constructor
-    intro h
-    rw [h]
-
-    unfold GroundAtom.toAtom
-    simp
-    intros sym terms
-    rw [GroundAtom.ext_iff]
-    constructor
-    apply sym
-    have : Function.Injective (List.map (Term.constant (τ := τ))) := by
-      rw [List.map_injective_iff]
-      intro _ _ term_eq
-      injection term_eq
-    apply this
-    exact terms
+    · intro h
+      rw [h]
+    · unfold GroundAtom.toAtom
+      simp only [Atom.mk.injEq, and_imp]
+      intros sym terms
+      rw [GroundAtom.ext_iff]
+      constructor
+      · apply sym
+      · have : Function.Injective (List.map (Term.constant (τ := τ))) := by
+          rw [List.map_injective_iff]
+          intro _ _ term_eq
+          injection term_eq
+        apply this
+        exact terms
 
   instance: Coe (GroundAtom τ) (Atom τ) where
     coe := GroundAtom.toAtom
 
-  lemma vars_empty (ga : GroundAtom τ) : ga.toAtom.vars = ∅ := by
+  lemma vars_empty (ga : GroundAtom τ) [DecidableEq τ.vars] : ga.toAtom.vars = ∅ := by
     unfold toAtom
     unfold Atom.vars
-    simp
+    simp only
     rw [List.foldl_union_empty]
-    simp
+    simp only [List.mem_map, forall_exists_index, and_imp, forall_apply_eq_imp_iff₂, true_and]
     intro _ _
     unfold Term.vars
     simp
 end GroundAtom
 
 namespace Atom
-  def toGroundAtom (a: Atom τ) (h: a.vars = ∅): GroundAtom τ :=
+  def toGroundAtom (a: Atom τ) [DecidableEq τ.vars] (h: a.vars = ∅) : GroundAtom τ :=
   {
     symbol:= a.symbol,
     atom_terms := List.map (fun ⟨t, t_in_a⟩ => t.toConstant (a.vars_empty_iff.mp h t t_in_a)) a.atom_terms.attach,
     term_length := by simp; apply a.term_length
   }
 
-  lemma toGroundAtom_isSelf (a: Atom τ) (h: a.vars = ∅): a = a.toGroundAtom h :=
+  lemma toGroundAtom_isSelf [DecidableEq τ.vars] (a: Atom τ) (h: a.vars = ∅): a = a.toGroundAtom h :=
   by
     unfold GroundAtom.toAtom
     unfold toGroundAtom
-    simp
+    simp only [List.map_map]
     rw [Atom.ext_iff]
-    simp
+    simp only [true_and]
     rw [vars_empty_iff] at h
-
     apply List.ext_get
-    simp
-    intro n h1 h2
-    simp
-
-    have h': ∀ (t : Term τ) (noVars : t.vars = ∅), t = t.toConstant noVars := by
-      intro t noVars
-      unfold Term.toConstant
-      cases t with
-      | constant c => simp
-      | variableDL v =>
-        unfold Term.vars at noVars
-        simp at noVars
-    apply h'
+    · simp
+    · intro n h1 h2
+      simp only [List.get_eq_getElem, List.getElem_map, List.getElem_attach, Function.comp_apply]
+      have h': ∀ (t : Term τ) (noVars : t.vars = ∅), t = t.toConstant noVars := by
+        intro t noVars
+        unfold Term.toConstant
+        cases t with
+        | constant c => simp
+        | variableDL v =>
+          unfold Term.vars at noVars
+          simp at noVars
+      apply h'
 end Atom
 
 namespace GroundRule
@@ -101,29 +118,28 @@ namespace GroundRule
   lemma eq_iff_toRule_eq (r1 r2: GroundRule τ): r1 = r2 ↔ r1.toRule = r2.toRule :=
   by
     constructor
-    intro h
-    rw [h]
+    · intro h
+      rw [h]
+    · unfold GroundRule.toRule
+      rw [GroundRule.ext_iff]
+      intro h
+      simp only [Rule.mk.injEq] at h
+      rcases h with ⟨head_eq, body_eq⟩
+      have inj_toAtom: Function.Injective (GroundAtom.toAtom (τ:= τ)) := by
+        unfold Function.Injective
+        intros a1 a2 h
+        rw [GroundAtom.eq_iff_toAtom_eq]
+        apply h
+      constructor
+      · unfold Function.Injective at inj_toAtom
+        apply inj_toAtom head_eq
+      · rw [← List.map_injective_iff] at inj_toAtom
+        apply inj_toAtom
+        exact body_eq
 
-    unfold GroundRule.toRule
-    rw [GroundRule.ext_iff]
-    intro h
-    simp at h
-    rcases h with ⟨head_eq, body_eq⟩
-    have inj_toAtom: Function.Injective (GroundAtom.toAtom (τ:= τ)) := by
-      unfold Function.Injective
-      intros a1 a2 h
-      rw [GroundAtom.eq_iff_toAtom_eq]
-      apply h
-    constructor
-    unfold Function.Injective at inj_toAtom
-    apply inj_toAtom head_eq
-    rw [← List.map_injective_iff] at inj_toAtom
-    apply inj_toAtom
-    exact body_eq
+  def bodySet [DecidableEq τ.constants] [DecidableEq τ.vars] [DecidableEq τ.relationSymbols] (r: GroundRule τ): Finset (GroundAtom τ) := List.toFinset r.body
 
-  def bodySet (r: GroundRule τ): Finset (GroundAtom τ) := List.toFinset r.body
-
-  lemma in_bodySet_iff_in_body (r: GroundRule τ) : ∀ a, a ∈ r.body ↔ a ∈ r.bodySet := by simp [bodySet]
+  lemma in_bodySet_iff_in_body [DecidableEq τ.constants] [DecidableEq τ.vars] [DecidableEq τ.relationSymbols] (r: GroundRule τ) : ∀ a, a ∈ r.body ↔ a ∈ r.bodySet := by simp [bodySet]
 end GroundRule
 
 namespace Grounding
@@ -137,18 +153,18 @@ namespace Grounding
   lemma applyTerm_preservesLength (g: Grounding τ) (a: Atom τ): (List.map g.applyTerm a.atom_terms).length = τ.relationArity a.symbol :=
   by
     rcases a with ⟨symbol, terms, term_length⟩
-    simp
+    simp only [List.length_map]
     rw [term_length]
 
   def applyAtom (g: Grounding τ) (a: Atom τ): Atom τ := {symbol := a.symbol, atom_terms := List.map g.applyTerm a.atom_terms, term_length := applyTerm_preservesLength g a}
 
-  lemma applyAtom_removesVars (a: Atom τ) (g: Grounding τ): (g.applyAtom a).vars = ∅ :=
+  lemma applyAtom_removesVars [DecidableEq τ.vars] (a: Atom τ) (g: Grounding τ): (g.applyAtom a).vars = ∅ :=
   by
     unfold applyAtom
     unfold Atom.vars
-    simp
+    simp only
     rw [List.foldl_union_empty]
-    simp
+    simp only [List.mem_map, forall_exists_index, and_imp, forall_apply_eq_imp_iff₂, true_and]
     intro x _
     unfold Term.vars
     unfold applyTerm
@@ -170,27 +186,27 @@ namespace Grounding
   lemma applyAtom'_on_GroundAtom_unchanged (g : Grounding τ) (ga : GroundAtom τ) : g.applyAtom' ga = ga := by
     unfold applyAtom'
     rw [GroundAtom.ext_iff]
-    simp [GroundAtom.toAtom]
+    simp only [GroundAtom.toAtom, List.map_map, true_and]
     apply List.ext_get
     · rw [List.length_map]
     · intro _ _ _
-      simp
+      simp only [List.get_eq_getElem, List.getElem_map, Function.comp_apply]
       rw [applyTerm'_on_constant_unchanged]
 
-  lemma applyAtom'_on_Atom_without_vars_unchanged (g : Grounding τ) (a : Atom τ) (noVars : a.vars = ∅) : g.applyAtom' a = a := by
+  lemma applyAtom'_on_Atom_without_vars_unchanged [DecidableEq τ.vars] (g : Grounding τ) (a : Atom τ) (noVars : a.vars = ∅) : g.applyAtom' a = a := by
     rw [a.toGroundAtom_isSelf noVars]
     rw [applyAtom'_on_GroundAtom_unchanged]
 
   def applyRule (r: Rule τ) (g: Grounding τ): Rule τ := {head := g.applyAtom r.head, body := List.map g.applyAtom r.body }
 
-  lemma applyRule_removesVars (r: Rule τ) (g: Grounding τ): (g.applyRule r).vars = ∅ := by
+  lemma applyRule_removesVars [DecidableEq τ.vars] (r: Rule τ) (g: Grounding τ): (g.applyRule r).vars = ∅ := by
     unfold applyRule
     unfold Rule.vars
-    simp
+    simp only [Finset.union_eq_empty]
     rw [applyAtom_removesVars]
-    simp
+    simp only [true_and]
     rw [List.foldl_union_empty]
-    simp
+    simp only [List.mem_map, forall_exists_index, and_imp, forall_apply_eq_imp_iff₂, true_and]
     intro a _
     apply applyAtom_removesVars
 
